finished proof that the test suite resulting from conversion into maximal io sequences is still complete and calculable

Experiments/Test_Suite_Calculation.thy
@@ -1339,6 +1339,24 @@ using passes_test_suite_completeness[OF calculate_test_suite_example_sufficient_
 
 
 
+definition calculate_test_suite_example_as_io_sequences :: "('a::linorder,'b::linorder,'c) fsm \<Rightarrow> nat \<Rightarrow> ('b \<times> 'c) list set" where
+  "calculate_test_suite_example_as_io_sequences M m = test_suite_to_io'_maximal M (calculate_test_suite_example M m)"
+
+lemma calculate_test_suite_example_as_io_sequences_completeness :
+  fixes M :: "('a::linorder,'b::linorder,'c) fsm"
+  assumes "observable M" 
+  and     "observable M'"
+  and     "inputs M' = inputs M"
+  and     "inputs M \<noteq> {}"
+  and     "completely_specified M"
+  and     "completely_specified M'"
+  and     "size M' \<le> m"
+shows     "(L M' \<subseteq> L M) \<longleftrightarrow> pass_io_set_maximal M' (calculate_test_suite_example_as_io_sequences M m)"
+  unfolding calculate_test_suite_example_as_io_sequences_def
+  using passes_test_suite_as_maximal_sequences_completeness[OF calculate_test_suite_example_sufficient_and_finite[OF \<open>observable M\<close> \<open>completely_specified M\<close> \<open>inputs M \<noteq> {}\<close>, of m] assms]
+  by assumption
+
+
 
 
 
@@ -1361,24 +1379,10 @@ value "case (calculate_test_suite_example m_ex_H 4) of
 value "case (calculate_test_suite_example m_ex_H 4) of
         (Test_Suite a b c d) \<Rightarrow>
           (image (\<lambda> (x,_) . image (\<lambda> xy . (xy, c xy)) (image (Pair x) (b x))) a)"
-                
-value "test_suite_to_io_code m_ex_H (calculate_test_suite_example m_ex_H 4)"
-value "(remove_proper_prefixes (test_suite_to_io_code m_ex_H (calculate_test_suite_example m_ex_H 4)))"
-value "card (remove_proper_prefixes (test_suite_to_io_code m_ex_H (calculate_test_suite_example m_ex_H 4)))"
-value "card (remove_proper_prefixes (test_suite_to_io_code m_ex_H (calculate_test_suite_example m_ex_H 5)))"
-value "card (remove_proper_prefixes (test_suite_to_io_code m_ex_H (calculate_test_suite_example m_ex_H 6)))"
 
+value "calculate_test_suite_example_as_io_sequences m_ex_H 4"
+value "calculate_test_suite_example_as_io_sequences m_ex_H 6"
 
-
-value "(remove_proper_prefixes (test_suite_to_io_code m_ex_9 (calculate_test_suite_example m_ex_9 4)))"
-value "card (remove_proper_prefixes (test_suite_to_io_code m_ex_9 (calculate_test_suite_example m_ex_9 4)))"
-value "card (remove_proper_prefixes (test_suite_to_io_code m_ex_9 (calculate_test_suite_example m_ex_9 5)))"
-value "card (remove_proper_prefixes (test_suite_to_io_code m_ex_9 (calculate_test_suite_example m_ex_9 6)))"
-
-
-
-definition example_calc :: "(integer\<times>integer) list set" where "example_calc = (remove_proper_prefixes (test_suite_to_io_code m_ex_DR (calculate_test_suite_example m_ex_DR (size m_ex_DR))))"
-
-export_code example_calc in Haskell module_name FSM
+export_code calculate_test_suite_example_as_io_sequences in Haskell module_name FSM
 
 end
